invariants for the naive algorithm

Scratch.thy
@@ -1,7 +1,7 @@
 (**)
 
 theory Scratch
-  imports "$AFP/RefineImperative_HOL/IICF/IICF"
+  imports "$AFP/Refine_Imperative_HOL/IICF/IICF"
 begin
   
   term "SPEC (\<lambda>x::nat. x \<in> {4,7,9})"
@@ -23,9 +23,10 @@ begin
     unfolding test_def
     apply refine_vcg by auto  
   
+  definition "i_test2 x\<^sub>0 \<equiv> \<lambda>(x,s). x\<ge>0 \<and> x\<^sub>0*5 = x*5+s"
   
   definition "test2 x\<^sub>0 \<equiv> do {
-    (_,s) \<leftarrow> WHILEIT (\<lambda>(x,s). x\<ge>0 \<and> x\<^sub>0*5 = x*5+s) (\<lambda>(x,s). x>0) (\<lambda>(x,s). do {
+    (_,s) \<leftarrow> WHILEIT (i_test2 x\<^sub>0) (\<lambda>(x,s). x>0) (\<lambda>(x,s). do {
       let s = s + 5;
       let x = x - 1;
       RETURN (x,s)
@@ -36,16 +37,61 @@ begin
   term "measure (nat o fst)"
     
   lemma "x\<ge>0 \<Longrightarrow> test2 x \<le> SPEC (\<lambda>r. r=x*5)"
-    unfolding test2_def
+    unfolding test2_def i_test2_def
     apply (refine_vcg WHILEIT_rule[where R="measure (nat o fst)"])  
     apply auto  
     done
-  
-  definition border :: "'a list \<Rightarrow> nat \<Rightarrow> nat" where "border s j \<equiv> undefined"    
       
+
+section\<open>Naive algorithm\<close>
+    
+subsection\<open>Invariants\<close>
+  definition "I_out_na t s \<equiv> \<lambda>(i,j(*_?*),found).
+    \<not>found \<and> j = 0 \<and> (\<forall>i' < i. \<not>is_substring_at t s i')
+    \<or> found \<and> is_substring_at t s i (*second part needed?*)"  
+  definition "I_in_na t s iout (*KMP should need jout, too*) \<equiv> \<lambda>(j,found).
+    j \<le> length s \<and> (\<forall>j' < j. t!(iout+j') = s!(j'))"  
+
+subsection\<open>Algorithm\<close>
+  definition "na t s \<equiv> do {
+    let i=0;
+    let j=0;
+    (_,_,found) \<leftarrow> WHILEI (I_out_na t s) (\<lambda>(i,j,found). i\<le>length t - length s \<and> \<not>found) (\<lambda>(i,j,found). do {
+      (j,found) \<leftarrow> WHILEI (I_in_na t s i) (\<lambda>(j,found). t!(i+j) = s!j \<and> \<not>found) (\<lambda>(j,found). do {
+        let j=j+1;
+        if j=length s then RETURN (j,True) else RETURN (j,False)
+      }) (j,found);
+      if \<not>found then do {
+        let i = i + 1;
+        let j = 0;
+        RETURN (i,j,False)
+      } else RETURN (i,j,True)
+    }) (i,j,False);
+
+    RETURN found
+  }"
+      
+  lemma "na t s \<le> SPEC (\<lambda>r. r \<longleftrightarrow> (\<exists>i. is_substring_at t s i))"
+    unfolding na_def I_out_na_def I_in_na_def
+    apply refine_vcg
+    apply vc_solve
+    using less_antisym apply blast
+    nitpick
+    
+    oops
+
+
+section\<open>Knuth–Morris–Pratt algorithm\<close>
+subsection\<open>Auxiliary definitions\<close>
+  definition border :: "'a list \<Rightarrow> nat \<Rightarrow> nat" where "border s j \<equiv> undefined"
+  
+  (*Todo: Properties*)
+
+subsection\<open>Invariants\<close>
   definition "I_outer \<equiv> \<lambda>(i,j,found). undefined"  
   definition "I_inner iout jout \<equiv> \<lambda>(j,found). undefined"  
-    
+
+subsection\<open>Algorithm\<close>
   definition "kmp t s \<equiv> do {
     let i=0; let j=0;
 
